\documentclass{article}
\usepackage[utf8]{inputenc}
\usepackage[dvipsnames]{xcolor}
\title{}

\begin{document}

\maketitle
\pagecolor{black}
\textcolor{white}{
\begin{center}
   The Gaussian Integral
    $$ \int_0^{\infty} e^{-x^2} \,dx = \frac{\sqrt{\pi}}{2} $$
    Swipe For EZ Proof \textcolor{red}{$\Rightarrow$}
\end{center}
\newpage
Let's start off with a simple $u$-substitution.
$$I = \int_0^{\infty} e^{-x^2} \,dx $$
$$x^2 \Rightarrow u \quad \quad 2x\,dx = \,du$$\\
\medskip{}
As $x = \sqrt{u}$, we have $\,dx = \frac{1}{2}u^{-\frac{1}{2}} \,du$
$$I = \frac{1}{2}\int_0^{\infty} u^{\frac{1}{2}-1} e^{-u} \,du = \frac{1}{2}\cdot \Gamma\left(\frac{1}{2}\right)$$
Recall from my last post that
$$\Gamma(s)\Gamma(1-s) = \frac{\pi}{\sin(\pi s)}$$
Let's plug in $s = \frac{1}{2}$ here to give us.
$$\bigg[\Gamma\left(\frac{1}{2}\right)\bigg]^2 = \frac{\pi}{\sin\left( \frac{\pi}{2}\right)} \Rightarrow \Gamma\left( \frac{1}{2}\right) = \sqrt{\pi}$$
$$I = \frac{1}{2} \cdot \Gamma\left( \frac{1}{2}\right)= \frac{\sqrt\pi}{2}$$
\newpage
$$\int_0^{\infty} e^{-x^2} \,dx = \frac{\sqrt{\pi}}{2}$$
\begin{center}
    For more, Follow
\end{center}
}


\end{document}

